Regex/NFA/Compile.lean
@@ -4,13 +4,10 @@ import Regex.NFA.Basic
 
 import Std.Data.Array.Lemmas
 
-namespace NFAa
+namespace NFA
 
--- TODO: remove once migration is complete
-open NFA
-
-def pushNode (nfa : NFAa) (node : NFA.Node) (inBounds : node.inBounds (nfa.nodes.size + 1)) :
-  { nfa' : NFAa // nfa.nodes.size < nfa'.nodes.size } :=
+def pushNode (nfa : NFA) (node : NFA.Node) (inBounds : node.inBounds (nfa.nodes.size + 1)) :
+  { nfa' : NFA // nfa.nodes.size < nfa'.nodes.size } :=
   let start := nfa.nodes.size
   let nodes := nfa.nodes.push node
   have inBounds := by
@@ -22,27 +19,27 @@ def pushNode (nfa : NFAa) (node : NFA.Node) (inBounds : node.inBounds (nfa.nodes
       have := nfa.inBounds ⟨i.val, h⟩
       apply Node.inBounds_of_inBounds_of_le this (Nat.le_succ _)
     case inr => exact inBounds
-  let nfa' : NFAa := ⟨nodes, ⟨start, by simp⟩, inBounds⟩
+  let nfa' : NFA := ⟨nodes, ⟨start, by simp⟩, inBounds⟩
 
   ⟨nfa', by simp⟩
 
 @[simp]
-theorem pushNode_size {nfa : NFAa} {node : Node} {inBounds : node.inBounds (nfa.nodes.size + 1)} :
+theorem pushNode_size {nfa : NFA} {node : Node} {inBounds : node.inBounds (nfa.nodes.size + 1)} :
   (nfa.pushNode node inBounds).val.nodes.size = nfa.nodes.size + 1 := by
   simp [pushNode]
 
-theorem pushNode_get_lt {nfa : NFAa} {node : Node} {inBounds : node.inBounds (nfa.nodes.size + 1)}
+theorem pushNode_get_lt {nfa : NFA} {node : Node} {inBounds : node.inBounds (nfa.nodes.size + 1)}
   (i : Nat) (h : i < nfa.nodes.size) :
   (nfa.pushNode node inBounds).val[i]'(Nat.lt_trans h (nfa.pushNode node inBounds).property) = nfa[i] := by
   simp [pushNode, get_eq_nodes_get]
   rw [Array.get_push_lt]
 
 @[simp]
-theorem pushNode_get_eq {nfa : NFAa} {node : Node} {inBounds : node.inBounds (nfa.nodes.size + 1)} :
+theorem pushNode_get_eq {nfa : NFA} {node : Node} {inBounds : node.inBounds (nfa.nodes.size + 1)} :
   (nfa.pushNode node inBounds).val[nfa.nodes.size] = node := by
   simp [pushNode, get_eq_nodes_get]
 
-theorem pushNode_get {nfa : NFAa} {node : Node} {inBounds : node.inBounds (nfa.nodes.size + 1)}
+theorem pushNode_get {nfa : NFA} {node : Node} {inBounds : node.inBounds (nfa.nodes.size + 1)}
   (i : Nat) (h : i < (nfa.pushNode node inBounds).val.nodes.size) :
   (nfa.pushNode node inBounds).val[i]'h = if h' : i < nfa.nodes.size then nfa[i]'h' else node := by
   simp at h
@@ -51,14 +48,14 @@ theorem pushNode_get {nfa : NFAa} {node : Node} {inBounds : node.inBounds (nfa.n
   | inr eq => simp [eq]
 
 @[simp]
-theorem pushNode_start_eq {nfa : NFAa} {node : Node} {inBounds : node.inBounds (nfa.nodes.size + 1)} :
+theorem pushNode_start_eq {nfa : NFA} {node : Node} {inBounds : node.inBounds (nfa.nodes.size + 1)} :
   (nfa.pushNode node inBounds).val.start.val = nfa.nodes.size := rfl
 
 /--
   Compile a Regex and append the resulting nodes to the NFA. The nodes will transition to `next` on match.
 -/
-def pushRegex (nfa : NFAa) (next : Fin nfa.nodes.size) :
-  Regex → { nfa' : NFAa // nfa.nodes.size < nfa'.nodes.size }
+def pushRegex (nfa : NFA) (next : Fin nfa.nodes.size) :
+  Regex → { nfa' : NFA // nfa.nodes.size < nfa'.nodes.size }
   | .empty => nfa.pushNode .fail rfl
   | .epsilon => nfa.pushNode (.epsilon next) (by simp [Node.inBounds]; exact Nat.lt_trans next.isLt (Nat.lt_succ_self _))
   | .char c => nfa.pushNode (.char c next) (by simp [Node.inBounds]; exact Nat.lt_trans next.isLt (Nat.lt_succ_self _))
@@ -148,8 +145,8 @@ def pushRegex (nfa : NFAa) (next : Fin nfa.nodes.size) :
 
     ⟨nfa', property⟩
 
--- TODO: push .*? for search
-def compile (r : Regex) : NFAa := done.pushRegex ⟨0, by decide⟩ r
+-- TODO: push .*? for search or simulate it with a loop
+def compile (r : Regex) : NFA := done.pushRegex ⟨0, by decide⟩ r
 
 -- Useful lemmas about the compilation
 theorem pushRegex.empty (eq : pushRegex nfa next .empty = result)
@@ -269,7 +266,7 @@ theorem pushRegex.star (eq : pushRegex nfa next (Regex.star r) = result)
       _ < _ := placeholder.property
       _ < _ := compiled.property
       _ = _ := by simp
-  let nfa' : NFAa := ⟨patched, ⟨nfa.nodes.size, isLt⟩, inBounds⟩
+  let nfa' : NFA := ⟨patched, ⟨nfa.nodes.size, isLt⟩, inBounds⟩
   have property :=
     calc
       _ < _ := placeholder.property
@@ -277,330 +274,5 @@ theorem pushRegex.star (eq : pushRegex nfa next (Regex.star r) = result)
       _ = nfa'.nodes.size := by simp
 
   exact motive placeholder compiled patched nfa' isLt inBounds property rfl rfl rfl rfl eq.symm
-
-end NFAa
-
-namespace NFA
-
-def NFA.addNode (nfa : NFA) (node : Node) :
-  { nfa' : NFA // nfa.nodes.size ≤ nfa'.nodes.size } :=
-  have isLt : nfa.nodes.size < (nfa.nodes.push node).size := by
-    simp [Array.size_push]
-  let start := nfa.nodes.size
-  let nfa' : NFA := ⟨nfa.nodes.push node, ⟨start, isLt⟩⟩
-
-  have property : nfa.nodes.size ≤ nfa'.nodes.size := by
-    simp
-    exact Nat.le_succ _
-
-  ⟨nfa', property⟩
-
-@[simp]
-theorem NFA.size_addNode {nfa : NFA} {node : Node} :
-  (nfa.addNode node).val.nodes.size = nfa.nodes.size + 1 := by
-  simp [NFA.addNode]
-
-theorem NFA.lt_size_addNode {nfa : NFA} {node : Node} :
-  nfa.nodes.size < (nfa.addNode node).val.nodes.size := (nfa.addNode node).val.start.isLt
-
-theorem NFA.get_lt_addNode {nfa : NFA} {node : Node} (h : i < nfa.nodes.size) :
-  (nfa.addNode node).val[i]'(Nat.lt_trans h lt_size_addNode) = nfa[i] :=
-  Array.get_push_lt _ _ _ h
-
-@[simp]
-theorem NFA.get?_addNode {nfa : NFA} {node : Node} :
-  (nfa.addNode node).val[(nfa.addNode node).val.start.val]? = some node := by
-  simp [NFA.addNode]
-  apply Array.get?_push_eq
-
-@[simp]
-theorem NFA.get_addNode {nfa : NFA} {node : Node} :
-  (nfa.addNode node).val[(nfa.addNode node).val.start.val] = node := by
-  simp [NFA.addNode]
-  apply Array.get_push_eq
-
-@[simp]
-theorem NFA.get_addNode' {nfa : NFA} {node : Node} :
-  (nfa.addNode node).val[nfa.nodes.size]'(NFA.lt_size_addNode) = node := by
-  have : nfa.nodes.size = (nfa.addNode node).val.start.val := by
-    simp [NFA.addNode]
-  simp [this]
-
-theorem NFA.start_addNode {nfa : NFA} {node : Node} {result : { nfa' : NFA // nfa.nodes.size ≤ nfa'.nodes.size }}
-  (eq : nfa.addNode node = result) :
-  result.val.start.val = nfa.nodes.size := by
-  rw [←eq]
-  simp [NFA.addNode]
-
-@[export lean_regex_nfa_compile_regex]
-def compile (r : Regex) : NFA :=
-  let result := loop r 0 init
-  result.val
-where
-  init : NFA := ⟨#[.done], ⟨0, Nat.zero_lt_succ _⟩⟩
-  /--
-    The main loop of the compilation.
-
-    It compiles the given regex into nodes that transitions to `next` on match.
-    Returned NFA contains the compiled nodes at the end and starts at the node
-    corresponding to the given regex.
-  -/
-  loop (r : Regex) (next : Nat) (nfa : NFA) : { nfa' // nfa.nodes.size ≤ nfa'.nodes.size } := match r with
-  | .empty => nfa.addNode .fail
-  | .epsilon => nfa.addNode (.epsilon next)
-  | .char c => nfa.addNode (.char c next)
-  | .alternate r₁ r₂ =>
-    -- TODO: it feels better to compile r₂ first to align with concat
-    let nfa₁ := loop r₁ next nfa
-    let start₁ := nfa₁.val.start
-    let nfa₂ := loop r₂ next nfa₁
-    let start₂ := nfa₂.val.start
-    let nfa' := nfa₂.val.addNode (.split start₁ start₂)
-
-    have property : nfa.nodes.size ≤ nfa'.val.nodes.size :=
-      calc nfa.nodes.size
-        _ ≤ nfa₁.val.nodes.size := nfa₁.property
-        _ ≤ nfa₂.val.nodes.size := nfa₂.property
-        _ ≤ nfa'.val.nodes.size := nfa'.property
-
-    ⟨nfa', property⟩
-  | .concat r₁ r₂ =>
-    let nfa₂ := loop r₂ next nfa
-    let nfa₁ := loop r₁ nfa₂.val.start nfa₂
-
-    have property : nfa.nodes.size ≤ nfa₁.val.nodes.size :=
-      calc nfa.nodes.size
-        _ ≤ nfa₂.val.nodes.size := nfa₂.property
-        _ ≤ nfa₁.val.nodes.size := nfa₁.property
-
-    ⟨nfa₁, property⟩
-  | .star r =>
-    -- We need to generate a placeholder node first. We use `fail` for it because
-    -- 1. We'll use the fact that `fail` is a minimal element when strengthening induction hypotheis;
-    -- 2. We want to make sure `done` does not appear except at the first node.
-    -- 3. variants without data are represented as a boxed integer so there is one less allocation.
-    -- TODO: check generated code
-    let nfa' := nfa.addNode .fail
-    let start := nfa'.val.start
-    let nfa'' := loop r start nfa'
-
-    have property : nfa.nodes.size ≤ nfa''.val.nodes.size :=
-      calc nfa.nodes.size
-        _ ≤ nfa'.val.nodes.size := nfa'.property
-        _ ≤ nfa''.val.nodes.size := nfa''.property
-    have isLt : start.val < nfa''.val.nodes.size :=
-      Nat.lt_of_lt_of_le nfa'.val.start.isLt nfa''.property
-
-    -- Patch the placeholder node
-    let target := nfa''.val.start
-    let nodes''' := nfa''.val.nodes.set ⟨start.val, isLt⟩ (.split target next)
-
-    -- TODO: maybe I should have used Fin.cast
-    have eq_size : nodes'''.size = nfa''.val.nodes.size := by simp
-    have isLt' : start.val < nodes'''.size := eq_size ▸ isLt
-    let nfa''' := ⟨nodes''', ⟨start.val, isLt'⟩⟩
-
-    have property' : nfa.nodes.size ≤ nfa'''.nodes.size := by
-      simp
-      exact property
-
-    ⟨nfa''', property'⟩
-
--- Useful lemmas about the compilation
-theorem compile.loop.empty (eq : compile.loop .empty next nfa = result)
-  {motive : result = nfa.addNode .fail → P} : P := by
-  simp [compile.loop] at eq
-  exact motive eq.symm
-
-theorem compile.loop.epsilon (eq : compile.loop .epsilon next nfa = result)
-  {motive : result = nfa.addNode (.epsilon next) → P} : P := by
-  simp [compile.loop] at eq
-  exact motive eq.symm
-
-theorem compile.loop.char (eq : compile.loop (.char c) next nfa = result)
-  {motive : result = nfa.addNode (.char c next) → P} : P := by
-  simp [compile.loop] at eq
-  exact motive eq.symm
-
-theorem compile.loop.alternate (eq : compile.loop (Regex.alternate r₁ r₂) next nfa = result)
-  {motive : ∀nfa₁ start₁ nfa₂ start₂ nfa' property,
-    nfa₁ = compile.loop r₁ next nfa →
-    start₁ = nfa₁.val.start →
-    nfa₂ = compile.loop r₂ next nfa₁ →
-    start₂ = nfa₂.val.start →
-    nfa' = nfa₂.val.addNode (.split start₁ start₂) →
-    result = ⟨nfa', property⟩ →
-    P
-  } : P := by
-  let nfa₁ := loop r₁ next nfa
-  let start₁ := nfa₁.val.start
-  let nfa₂ := loop r₂ next nfa₁
-  let start₂ := nfa₂.val.start
-  let nfa' := nfa₂.val.addNode (.split start₁ start₂)
-
-  have property : nfa.nodes.size ≤ nfa'.val.nodes.size :=
-    calc nfa.nodes.size
-      _ ≤ nfa₁.val.nodes.size := nfa₁.property
-      _ ≤ nfa₂.val.nodes.size := nfa₂.property
-      _ ≤ nfa'.val.nodes.size := nfa'.property
-
-  have : result = ⟨nfa', property⟩ := by
-    simp [eq.symm, compile.loop]
-  exact motive nfa₁ start₁ nfa₂ start₂ nfa' property rfl rfl rfl rfl rfl this
-
-theorem compile.loop.concat (eq : compile.loop (Regex.concat r₁ r₂) next nfa = result)
-  {motive : ∀nfa₂ nfa₁ property,
-    nfa₂ = compile.loop r₂ next nfa →
-    nfa₁ = compile.loop r₁ nfa₂.val.start nfa₂ →
-    result = ⟨nfa₁, property⟩ →
-    P
-  } : P := by
-  let nfa₂ := loop r₂ next nfa
-  let nfa₁ := loop r₁ nfa₂.val.start nfa₂
-
-  have property : nfa.nodes.size ≤ nfa₁.val.nodes.size :=
-    calc nfa.nodes.size
-      _ ≤ nfa₂.val.nodes.size := nfa₂.property
-      _ ≤ nfa₁.val.nodes.size := nfa₁.property
-
-  have : result = ⟨nfa₁, property⟩ := by
-    simp [eq.symm, compile.loop]
-  exact motive nfa₂ nfa₁ property rfl rfl this
-
-theorem compile.loop.star (eq : compile.loop (Regex.star r) next nfa = result)
-  {motive : ∀nfa' start nfa'' nodes''' nfa''' isLt isLt' property',
-    nfa' = nfa.addNode .fail →
-    start = nfa'.val.start →
-    nfa'' = compile.loop r start nfa' →
-    nodes''' = nfa''.val.nodes.set ⟨start.val, isLt⟩ (.split nfa''.val.start next) →
-    nfa''' = ⟨nodes''', ⟨start.val, isLt'⟩⟩ →
-    result = ⟨nfa''', property'⟩ →
-    P
-  } : P := by
-  let nfa' := nfa.addNode .fail
-  let start := nfa'.val.start
-  let nfa'' := loop r start nfa'
-
-  have property : nfa.nodes.size ≤ nfa''.val.nodes.size :=
-    calc nfa.nodes.size
-      _ ≤ nfa'.val.nodes.size := nfa'.property
-      _ ≤ nfa''.val.nodes.size := nfa''.property
-  have isLt : start.val < nfa''.val.nodes.size :=
-    Nat.lt_of_lt_of_le nfa'.val.start.isLt nfa''.property
-
-  -- Patch the placeholder node
-  let nodes''' := nfa''.val.nodes.set ⟨start.val, isLt⟩ (.split nfa''.val.start next)
-
-  have eq_size : nodes'''.size = nfa''.val.nodes.size := by simp
-  have isLt' : start.val < nodes'''.size := eq_size ▸ isLt
-  let nfa''' : NFA := ⟨nodes''', ⟨start.val, isLt'⟩⟩
-
-  have property' : nfa.nodes.size ≤ nfa'''.nodes.size := by
-    simp
-    exact property
-
-  have : result = ⟨nfa''', property'⟩ := by
-    simp [eq.symm, compile.loop]
-  exact motive nfa' start nfa'' nodes''' nfa''' isLt isLt' property' rfl rfl rfl rfl rfl this
-
-theorem compile.loop.inBounds (eq : compile.loop r next nfa = result)
-  (h₁ : next < nfa.nodes.size) (h₂ : nfa.inBounds) :
-  result.val.inBounds := by
-  induction r generalizing next nfa with
-  | empty | epsilon | char =>
-    try apply compile.loop.empty eq
-    try apply compile.loop.epsilon eq
-    try apply compile.loop.char eq
-
-    intro eq i
-    subst eq
-    have h' : next < nfa.nodes.size + 1 := Nat.lt_trans h₁ (Nat.lt_succ_self _)
-
-    cases Nat.lt_or_ge i nfa.nodes.size with
-    | inl lt =>
-      simp [NFA.get_lt_addNode lt]
-      exact Node.inBounds_of_inBounds_of_le (h₂ ⟨i, lt⟩) (Nat.le_succ _)
-    | inr ge =>
-      let lt := i.isLt
-      simp only [NFA.addNode, Array.size_push] at lt
-      have : i = nfa.nodes.size := Nat.eq_of_ge_of_lt ge lt
-      simp [this]
-      try simp [NFA.addNode]
-      try exact Node.inBounds.epsilon h'
-      try exact Node.inBounds.char h'
-  | alternate r₁ r₂ ih₁ ih₂ =>
-    apply compile.loop.alternate eq
-    intro nfa₁ start₁ nfa₂ start₂ nfa' property eq₁ _ eq₃ _ eq₅ eq i
-
-    have ih : i < nfa₂.val.nodes.size → result.val[i].inBounds result.val.nodes.size := by
-      intro h
-      simp [eq, eq₅]
-      simp [NFA.get_lt_addNode h]
-      have ih₁ := ih₁ eq₁.symm h₁ h₂
-      have ih₂ := ih₂ eq₃.symm (Nat.lt_of_lt_of_le h₁ nfa₁.property) ih₁
-      exact Node.inBounds_of_inBounds_of_le (ih₂ ⟨i, h⟩) (Nat.le_succ _)
-
-    cases Nat.lt_or_ge i nfa₂.val.nodes.size with
-    | inl lt => exact ih lt
-    | inr ge =>
-      let lt := i.isLt
-      simp only [eq, eq₅, NFA.addNode, Array.size_push] at lt
-      have : i = nfa₂.val.nodes.size := Nat.eq_of_ge_of_lt ge lt
-      simp [eq, eq₅, this]
-      apply Node.inBounds.split
-      . exact Nat.lt_trans start₁.isLt (Nat.lt_of_le_of_lt nfa₂.property (Nat.lt_succ_self _))
-      . exact Nat.lt_trans start₂.isLt (Nat.lt_succ_self _)
-  | concat r₁ r₂ ih₁ ih₂ =>
-    apply compile.loop.concat eq
-    intro nfa₂ nfa₁ property eq₂ eq₁ eq
-    simp [eq]
-    apply ih₁ eq₁.symm nfa₂.val.start.isLt
-    apply ih₂ eq₂.symm h₁ h₂
-  | star r ih =>
-    apply compile.loop.star eq
-    intro nfa' start nfa'' nodes''' nfa''' isLt isLt' property'
-      eq₁ _ eq₃ eq₄ eq₅ eq i
-
-    have eqsize : result.val.nodes.size = nfa''.val.nodes.size := by
-      simp [eq, eq₅, eq₄]
-    have h' : i < nfa''.val.nodes.size :=
-      calc
-        i < result.val.nodes.size := i.isLt
-        _ = _ := eqsize
-    have inBounds' : nfa'.val.inBounds := by
-      simp [eq₁]
-      intro i
-      cases Nat.lt_or_ge i nfa.nodes.size with
-      | inl lt =>
-        simp [NFA.get_lt_addNode lt]
-        exact Node.inBounds_of_inBounds_of_le (h₂ ⟨i, lt⟩) (Nat.le_succ _)
-      | inr ge =>
-        let lt := i.isLt
-        simp only [NFA.addNode, Array.size_push] at lt
-        have : i = nfa.nodes.size := Nat.eq_of_ge_of_lt ge lt
-        simp [this]
-    have ih := ih eq₃.symm start.isLt inBounds'
-
-    simp [eq, eq₅, NFA.eq_get, eq₄, Array.get_set, h']
-    split
-    . apply Node.inBounds.split
-      . exact nfa''.val.start.isLt
-      . exact Nat.lt_of_lt_of_le h₁ (Nat.le_trans nfa'.property nfa''.property)
-    . exact ih (i.cast eqsize)
-
-theorem compile.init.inBounds : compile.init.inBounds := by
-  intro i
-  simp [NFA.eq_get, init]
-  match i with
-  | ⟨0, _⟩ =>
-    show Node.done.inBounds 1
-    simp [Node.inBounds]
-  | ⟨i + 1, isLt⟩ =>
-    simp [init] at isLt
-    contradiction
-
-theorem compile.inBounds (eq : compile r = result) : result.inBounds := by
-  simp [eq.symm, compile]
-  exact compile.loop.inBounds rfl (by decide) compile.init.inBounds
 
 end NFA
