Regex/NFA/VM/Basic.lean
@@ -334,77 +334,8 @@ theorem NodeSet.merge_get {ns₁ ns₂ : NodeSet n} {x : Fin n} :
   apply this
 termination_by go _ => n - i
 
-open NFA
-
 -- TODO: check if the modifications don't cause copying
-def εClosureTR (nfa : NFA) (inBounds : nfa.inBounds)
-  (visited : NodeSet nfa.nodes.size) (stack : Array (Fin nfa.nodes.size)) :
-  NodeSet nfa.nodes.size :=
-  if hemp : stack.isEmpty then
-    visited
-  else
-    let i := stack.back' hemp
-    let stack' := stack.pop
-    have : stack'.size < stack.size := Array.lt_size_of_pop_of_not_empty _ hemp
-    if hvis : visited.get i then
-      εClosureTR nfa inBounds visited stack'
-    else
-      let visited' := visited.set i
-      have : visited'.count_unset < visited.count_unset := visited.lt_count_unset i.isLt hvis
-      have inBounds' := inBounds i
-      let stack'' :=
-        match hn : nfa[i] with
-        | .epsilon next =>
-          have h : next < nfa.nodes.size := by
-            rw [hn] at inBounds'
-            simp [Node.inBounds] at inBounds'
-            exact inBounds'
-
-          stack'.push ⟨next, h⟩
-        | .split next₁ next₂ =>
-          have h₁ : next₁ < nfa.nodes.size := by
-            rw [hn] at inBounds'
-            simp [Node.inBounds] at inBounds'
-            exact inBounds'.left
-          have h₂ : next₂ < nfa.nodes.size := by
-            rw [hn] at inBounds'
-            simp [Node.inBounds] at inBounds'
-            exact inBounds'.right
-
-          (stack'.push ⟨next₁, h₁⟩).push ⟨next₂, h₂⟩
-        | _ => stack'
-      εClosureTR nfa inBounds visited' stack''
-termination_by _ => (visited.count_unset, stack.size)
-
-def charStepTR (nfa : NFA) (inBounds : nfa.inBounds) (c : Char) (init : NodeSet nfa.nodes.size) :
-  NodeSet nfa.nodes.size := go nfa inBounds c init .empty 0 (Nat.zero_le _)
-where
-  go (nfa : NFA) (inBounds : nfa.inBounds) (c : Char) (init : NodeSet nfa.nodes.size)
-    (accum : NodeSet nfa.nodes.size) (i : Nat) (hle : i ≤ nfa.nodes.size) :
-    NodeSet nfa.nodes.size :=
-    if h : i = nfa.nodes.size then
-      accum
-    else
-      have hlt : i < nfa.nodes.size := Nat.lt_of_le_of_ne hle h
-      let accum := if init.get ⟨i, hlt⟩ then
-        match hn : nfa[i] with
-        | .char c' next =>
-          if c = c' then
-            have : next < nfa.nodes.size := by
-              have := inBounds ⟨i, hlt⟩
-              simp [hn, Node.inBounds] at this
-              exact this
-            -- TODO: reuse visited and stack
-            accum.merge (εClosureTR nfa inBounds .empty #[⟨next, this⟩])
-          else
-            accum
-        | _ => accum
-      else accum
-      go nfa inBounds c init accum (i + 1) hlt
-termination_by go _ => nfa.nodes.size - i
-
--- TODO: check if the modifications don't cause copying
-def εClosureTRa (nfa : NFAa) (visited : NodeSet nfa.nodes.size) (stack : Array (Fin nfa.nodes.size)) :
+def εClosureTRa (nfa : NFA) (visited : NodeSet nfa.nodes.size) (stack : Array (Fin nfa.nodes.size)) :
   NodeSet nfa.nodes.size :=
   if hemp : stack.isEmpty then
     visited
@@ -442,10 +373,10 @@ def εClosureTRa (nfa : NFAa) (visited : NodeSet nfa.nodes.size) (stack : Array 
       εClosureTRa nfa visited' stack''
 termination_by _ => (visited.count_unset, stack.size)
 
-def charStepTRa (nfa : NFAa) (c : Char) (init : NodeSet nfa.nodes.size) :
+def charStepTRa (nfa : NFA) (c : Char) (init : NodeSet nfa.nodes.size) :
   NodeSet nfa.nodes.size := go nfa c init .empty 0 (Nat.zero_le _)
 where
-  go (nfa : NFAa) (c : Char) (init : NodeSet nfa.nodes.size)
+  go (nfa : NFA) (c : Char) (init : NodeSet nfa.nodes.size)
     (accum : NodeSet nfa.nodes.size) (i : Nat) (hle : i ≤ nfa.nodes.size) :
     NodeSet nfa.nodes.size :=
     if h : i = nfa.nodes.size then
@@ -474,26 +405,13 @@ end NFA.VM
 open NFA.VM
 
 @[export lean_regex_nfa_match]
-def NFA.NFA.match (nfa : NFA) (inBounds : nfa.inBounds) (s : String) : Bool :=
-  let ns := εClosureTR nfa inBounds .empty #[nfa.start]
-  let ns := go nfa inBounds s.iter ns
-  -- This assumes that the first node is the accepting node
-  ns.get ⟨0, nfa.zero_lt_size⟩
-where
-  go (nfa : NFA) (inBounds : nfa.inBounds) (iter : String.Iterator) (ns : NodeSet nfa.nodes.size) : NodeSet nfa.nodes.size :=
-    if iter.atEnd then
-      ns
-    else
-      let ns' := charStepTR nfa inBounds iter.curr ns
-      go nfa inBounds iter.next ns'
-
-def NFAa.match (nfa : NFAa) (s : String) : Bool :=
+def NFA.match (nfa : NFA) (s : String) : Bool :=
   let ns := εClosureTRa nfa .empty #[nfa.start]
   let ns := go nfa s.iter ns
   -- This assumes that the first node is the accepting node
   ns.get ⟨0, nfa.zero_lt_size⟩
 where
-  go (nfa : NFAa) (iter : String.Iterator) (ns : NodeSet nfa.nodes.size) : NodeSet nfa.nodes.size :=
+  go (nfa : NFA) (iter : String.Iterator) (ns : NodeSet nfa.nodes.size) : NodeSet nfa.nodes.size :=
     if iter.atEnd then
       ns
     else
