RegexCorrectness/NFA/Basic.lean
@@ -15,64 +15,22 @@ def Node.εStep (n : Node) : Set Nat :=
   | Node.split next₁ next₂ => {next₁, next₂}
   | _ => ∅
 
-theorem lt_of_inBounds_of_charStep {nfa : NFA} {i j : Nat} {c : Char} {h : i < nfa.nodes.size}
-  (inBounds : nfa.inBounds) (mem : j ∈ nfa[i].charStep c) :
-  j < nfa.nodes.size := by
-  unfold Node.charStep at mem
-  split at mem <;> try contradiction
-  next next eq =>
-    split at mem <;> try contradiction
-    simp at mem
-    rw [mem]
-    have := inBounds ⟨i, h⟩
-    simp [eq, Node.inBounds] at this
-    exact this
-
-theorem lt_of_inBounds_of_εStep {nfa : NFA} {i j : Nat} {h : i < nfa.nodes.size}
-  (inBounds : nfa.inBounds) (mem : j ∈ nfa[i].εStep) :
-  j < nfa.nodes.size := by
-  unfold Node.εStep at mem
-  split at mem <;> try contradiction
-  next next eq =>
-    have := inBounds ⟨i, h⟩
-    simp [eq, Node.inBounds] at this
-    simp at mem
-    rw [mem]
-    exact this
-  next next₁ next₂ eq =>
-    have := inBounds ⟨i, h⟩
-    simp [eq, Node.inBounds] at this
-    simp at mem
-    cases mem with
-    | inl eq₁ =>
-      rw [eq₁]
-      exact this.left
-    | inr eq₂ =>
-      rw [eq₂]
-      exact this.right
-
-end NFA
-
-namespace NFAa
-
-open NFA
-
-def charStep (nfa : NFAa) (i : Nat) (c : Char) : Set Nat :=
+def charStep (nfa : NFA) (i : Nat) (c : Char) : Set Nat :=
   if h : i < nfa.nodes.size then
     nfa[i].charStep c
   else ∅
 
-def εStep (nfa : NFAa) (i : Nat) : Set Nat :=
+def εStep (nfa : NFA) (i : Nat) : Set Nat :=
   if h : i < nfa.nodes.size then
     nfa[i].εStep
   else ∅
 
-theorem charStep_of_charStep {nfa : NFAa} {i : Nat} {c : Char} {h : i < nfa.nodes.size}
+theorem charStep_of_charStep {nfa : NFA} {i : Nat} {c : Char} {h : i < nfa.nodes.size}
   (mem : j ∈ nfa[i].charStep c) :
   j ∈ nfa.charStep i c := by
   simp [charStep, h, mem]
 
-theorem εStep_of_εStep {nfa : NFAa} {i : Nat} {h : i < nfa.nodes.size}
+theorem εStep_of_εStep {nfa : NFA} {i : Nat} {h : i < nfa.nodes.size}
   (mem : j ∈ nfa[i].εStep) :
   j ∈ nfa.εStep i := by
   simp [εStep, h, mem]
@@ -93,19 +51,19 @@ theorem lt_of_inBounds_of_εStep {node : Node} {j k : Nat}
     try cases mem <;>
     simp [*]
 
-theorem lt_of_εStep {nfa : NFAa} {i j : Nat} {h : i < nfa.nodes.size}
+theorem lt_of_εStep {nfa : NFA} {i j : Nat} {h : i < nfa.nodes.size}
   (mem : j ∈ nfa[i].εStep) : j < nfa.nodes.size := by
   have inBounds := nfa.inBounds ⟨i, h⟩
   simp [get_eq_nodes_get] at mem
   exact lt_of_inBounds_of_εStep inBounds mem
 
-theorem lt_of_charStep {nfa : NFAa} {i j : Nat} {h : i < nfa.nodes.size}
+theorem lt_of_charStep {nfa : NFA} {i j : Nat} {h : i < nfa.nodes.size}
   (mem : j ∈ nfa[i].charStep c) : j < nfa.nodes.size := by
   have inBounds := nfa.inBounds ⟨i, h⟩
   simp [get_eq_nodes_get] at mem
   exact lt_of_inBounds_of_charStep inBounds mem
 
--- def step (nfa : NFAa) (i : Fin nfa.nodes.size) (c : Option Char) : Set (Fin nfa.nodes.size) :=
+-- def step (nfa : NFA) (i : Fin nfa.nodes.size) (c : Option Char) : Set (Fin nfa.nodes.size) :=
 --   match c, nfa[i], nfa.inBounds i with
 --   | .some c, .char c' next, inBounds =>
 --     if c == c' then {⟨next, Node.lt_of_inBounds.char inBounds⟩} else ∅
@@ -115,7 +73,7 @@ theorem lt_of_charStep {nfa : NFAa} {i j : Nat} {h : i < nfa.nodes.size}
 --     {⟨next₁, lt.left⟩, ⟨next₂, lt.right⟩}
 --   | _, _, _ => ∅
 
--- theorem charStep_cases {nfa : NFAa} {i j : Fin nfa.nodes.size} {c : Char}
+-- theorem charStep_cases {nfa : NFA} {i j : Fin nfa.nodes.size} {c : Char}
 --   (h : j ∈ nfa.step i (.some c)) (char : nfa[i.val] = Node.char c j.val → motive)
 --   : motive := by
 --   simp [step] at h
@@ -124,7 +82,7 @@ theorem lt_of_charStep {nfa : NFAa} {i j : Nat} {h : i < nfa.nodes.size}
 --     apply char
 --     simp [eqn, eqc, h]
 
--- theorem εStep_cases {nfa : NFAa} {i j : Fin nfa.nodes.size}
+-- theorem εStep_cases {nfa : NFA} {i j : Fin nfa.nodes.size}
 --   (h : j ∈ nfa.step i .none)
 --   (epsilon : nfa[i.val] = Node.epsilon j.val → motive)
 --   (split : ∀ next₁ next₂, nfa[i.val] = Node.split next₁ next₂ → j.val = next₁ ∨ j.val = next₂ → motive) :
@@ -138,7 +96,7 @@ theorem lt_of_charStep {nfa : NFAa} {i j : Nat} {h : i < nfa.nodes.size}
 --     apply split next₁ next₂ eqn
 --     cases h <;> simp [*]
 
--- theorem step_cases {nfa : NFAa} {i j : Fin nfa.nodes.size} (h : j ∈ nfa.step i c)
+-- theorem step_cases {nfa : NFA} {i j : Fin nfa.nodes.size} (h : j ∈ nfa.step i c)
 --   (char : ∀ c', c = .some c' → nfa[i.val] = Node.char c' j.val → motive)
 --   (epsilon : c = none → nfa[i.val] = Node.epsilon j.val → motive)
 --   (split : ∀ next₁ next₂, c = none → nfa[i.val] = Node.split next₁ next₂ →
@@ -148,4 +106,4 @@ theorem lt_of_charStep {nfa : NFAa} {i j : Nat} {h : i < nfa.nodes.size}
 --   | none => apply εStep_cases h (epsilon rfl) (fun next₁ next₂ => split _ _ rfl)
 --   | some c' => apply charStep_cases h (char c' rfl)
 
-end NFAa
+end NFA
