RegexCorrectness/NFA/VM/Correctness.lean
@@ -79,516 +79,6 @@ theorem mem_εStep_iff_εClosure_sub {nfa : NFA} {S : Set Nat} :
   ∀ i ∈ S, nfa.εClosure i ⊆ S := by
   apply Iff.intro
   . intro assm i mem
-    simp [Set.subset_def]
-    intro k cls
-    induction cls with
-    | base => exact mem
-    | @step i j k step _ ih =>
-      cases Nat.decLt i nfa.nodes.size with
-      | isTrue lt =>
-        simp [getElem?_pos nfa i lt, Option.εStep] at step
-        exact ih (assm i mem lt j step)
-      | isFalse nlt => simp [getElem?_neg nfa i nlt, Option.εStep] at step
-  . intro assm i mem lt j step
-    apply Set.mem_of_mem_of_subset _ (assm i mem)
-    have step' : j ∈ nfa[i]?.εStep := by
-      simp [getElem?_pos nfa i lt, Option.εStep, step]
-    exact NFA.εClosure.step step' .base
-
-theorem εClosureTR_spec {i : Fin nfa.nodes.size} {inBounds : nfa.inBounds} :
-  ∀ j, (εClosureTR nfa inBounds .empty #[i]).get j ↔ j.val ∈ nfa.εClosure i := by
-  let inv (visited : NodeSet nfa.nodes.size) (stack : Array (Fin nfa.nodes.size)) : Prop :=
-    (visited.get i ∨ i ∈ stack) ∧
-    (∀ i j, visited.get i → j.val ∈ nfa[i].εStep → visited.get j ∨ j ∈ stack) ∧
-    (∀ j, (visited.get j ∨ j ∈ stack) → j.val ∈ nfa.εClosure i)
-
-  let rec go (visited : NodeSet nfa.nodes.size) (stack : Array (Fin nfa.nodes.size))
-    (inv₀ : inv visited stack) : inv (εClosureTR nfa inBounds visited stack) #[] := by
-    unfold εClosureTR
-    split
-    case inl hemp =>
-      have : stack = #[] := (Array.isEmpty_iff).mp hemp
-      exact this ▸ inv₀
-    case inr hemp =>
-      set n := stack.back' hemp with hn
-      set stack' := stack.pop with hs'
-      have : stack.pop.size < stack.size :=
-        Array.lt_size_of_pop_of_not_empty _ hemp
-      cases hvis : visited.get n with
-      | true =>
-        simp [hvis]
-        have inv' : inv visited stack.pop := by
-          apply And.intro
-          . cases inv₀.1 with
-            | inl vis => exact Or.inl vis
-            | inr stk =>
-              cases Nat.decEq i n with
-              | isTrue eq =>
-                have : i = n := Fin.eq_of_val_eq eq
-                exact Or.inl (this ▸ hvis)
-              | isFalse neq =>
-                have : i ≠ n := Fin.ne_of_val_ne neq
-                exact Or.inr (Array.mem_pop _ _ _ stk this)
-          . apply And.intro
-            . intro i j mem step
-              cases inv₀.2.1 i j mem step with
-              | inl vis => exact Or.inl vis
-              | inr stk =>
-                cases decEq j n with
-                | isTrue eq => exact Or.inl (eq ▸ hvis)
-                | isFalse neq => exact Or.inr (Array.mem_pop _ _ _ stk neq)
-            . intro j mem
-              cases mem with
-              | inl vis => exact inv₀.2.2 j (.inl vis)
-              | inr stk =>
-                have : j ∈ stack := Array.mem_of_mem_pop _ _ stk
-                exact inv₀.2.2 j (.inr this)
-        have ih := go visited stack.pop inv'
-        simp at ih
-        exact ih
-      | false =>
-        have : (visited.set n).count_unset < visited.count_unset :=
-          visited.lt_count_unset n.isLt (by simp [hvis])
-        have inBounds' := inBounds n
-        simp [hvis]
-        split
-        next next eqEps =>
-          have h : next < nfa.nodes.size := by
-            rw [hn] at inBounds'
-            simp [eqEps, Node.inBounds] at inBounds'
-            exact inBounds'
-
-          set stack'' := stack'.push ⟨next, h⟩ with hs''
-          have inv' : inv (visited.set n) stack'' := by
-            apply And.intro
-            . cases inv₀.1 with
-              | inl vis => simp [NodeSet.get_set_set vis]
-              | inr stk =>
-                cases Array.mem_pop_or_eq_of_mem _ _ hemp stk with
-                | inl stk => exact Or.inr ((Array.mem_push _ _ _).mpr (.inl stk))
-                | inr eq => simp [hn, eq]
-            . apply And.intro
-              . intro i j mem step
-                rw [NodeSet.get_set] at mem
-                split at mem
-                case inl eq =>
-                  simp [eq.symm, eqEps, Node.εStep] at step
-                  exact Or.inr ((Array.mem_push _ _ _).mpr (.inr (Fin.eq_of_val_eq step)))
-                case inr neq =>
-                  cases inv₀.2.1 i j mem step with
-                  | inl vis => simp [NodeSet.get_set_set vis]
-                  | inr stk =>
-                    cases Array.mem_pop_or_eq_of_mem _ _ hemp stk with
-                    | inl stk => exact Or.inr ((Array.mem_push _ _ _).mpr (.inl stk))
-                    | inr eq => simp [hn, eq]
-              . intro j mem
-                cases mem with
-                | inl vis =>
-                  rw [NodeSet.get_set] at vis
-                  split at vis
-                  case inl eq =>
-                    rw [←eq]
-                    exact inv₀.2.2 n (.inr (Array.mem_back' hemp))
-                  case inr _ => exact inv₀.2.2 j (.inl vis)
-                | inr stk =>
-                  cases (Array.mem_push _ _ _).mp stk with
-                  | inl stk =>
-                    have : j ∈ stack := Array.mem_of_mem_pop _ _ stk
-                    exact inv₀.2.2 j (.inr this)
-                  | inr eq =>
-                    simp [eq]
-                    have : n.val ∈ nfa.εClosure i := inv₀.2.2 n (.inr (Array.mem_back' hemp))
-                    exact εClosure_snoc n.isLt this (by simp [Node.εStep, eqEps])
-          have ih := go (visited.set n) stack'' inv'
-          simp at ih
-          exact ih
-        next next₁ next₂ eqSplit =>
-          rw [hn] at inBounds'
-          simp [eqSplit, Node.inBounds] at inBounds'
-          have h₁ : next₁ < nfa.nodes.size := inBounds'.left
-          have h₂ : next₂ < nfa.nodes.size := inBounds'.right
-
-          set stack'' := (stack'.push ⟨next₁, h₁⟩).push ⟨next₂, h₂⟩ with hs''
-          have inv' : inv (visited.set n) stack'' := by
-            apply And.intro
-            . cases inv₀.1 with
-              | inl vis => simp [NodeSet.get_set_set vis]
-              | inr stk =>
-                cases Array.mem_pop_or_eq_of_mem _ _ hemp stk with
-                | inl stk =>
-                  apply Or.inr
-                  apply (Array.mem_push _ _ _).mpr
-                  apply Or.inl
-                  apply (Array.mem_push _ _ _).mpr
-                  exact Or.inl stk
-                | inr eq => simp [hn, eq]
-            . apply And.intro
-              . intro i j mem step
-                rw [NodeSet.get_set] at mem
-                split at mem
-                case inl eq =>
-                  simp [eq.symm, eqSplit, Node.εStep] at step
-                  cases step with
-                  | inl eq₁ =>
-                    apply Or.inr
-                    apply (Array.mem_push _ _ _).mpr
-                    apply Or.inl
-                    apply (Array.mem_push _ _ _).mpr
-                    apply Or.inr
-                    apply Fin.eq_of_val_eq
-                    exact eq₁
-                  | inr eq₂ =>
-                    apply Or.inr
-                    apply (Array.mem_push _ _ _).mpr
-                    apply Or.inr
-                    apply Fin.eq_of_val_eq
-                    exact eq₂
-                case inr neq =>
-                  cases inv₀.2.1 i j mem step with
-                  | inl vis => simp [NodeSet.get_set_set vis]
-                  | inr stk =>
-                    cases Array.mem_pop_or_eq_of_mem _ _ hemp stk with
-                    | inl stk =>
-                      apply Or.inr
-                      apply (Array.mem_push _ _ _).mpr
-                      apply Or.inl
-                      apply (Array.mem_push _ _ _).mpr
-                      exact Or.inl stk
-                    | inr eq => simp [hn, eq]
-              . intro j mem
-                cases mem with
-                | inl vis =>
-                  rw [NodeSet.get_set] at vis
-                  split at vis
-                  case inl eq =>
-                    rw [←eq]
-                    exact inv₀.2.2 n (.inr (Array.mem_back' hemp))
-                  case inr _ => exact inv₀.2.2 j (.inl vis)
-                | inr stk =>
-                  cases (Array.mem_push _ _ _).mp stk with
-                  | inl stk =>
-                    cases (Array.mem_push _ _ _).mp stk with
-                    | inl stk =>
-                      have : j ∈ stack := Array.mem_of_mem_pop _ _ stk
-                      exact inv₀.2.2 j (.inr this)
-                    | inr eq =>
-                      simp [eq]
-                      have : n.val ∈ nfa.εClosure i := inv₀.2.2 n (.inr (Array.mem_back' hemp))
-                      exact εClosure_snoc n.isLt this (by simp [Node.εStep, eqSplit])
-                  | inr eq =>
-                    simp [eq]
-                    have : n.val ∈ nfa.εClosure i := inv₀.2.2 n (.inr (Array.mem_back' hemp))
-                    exact εClosure_snoc n.isLt this (by simp [Node.εStep, eqSplit])
-          have ih := go (visited.set n) stack'' inv'
-          simp at ih
-          exact ih
-        next hne₁ hne₂ =>
-          have inv' : inv (visited.set n) stack.pop := by
-            apply And.intro
-            . cases inv₀.1 with
-              | inl vis =>
-                rw [NodeSet.get_set_set vis]
-                simp
-              | inr stk =>
-                cases Array.mem_pop_or_eq_of_mem _ _ hemp stk with
-                | inl stk => exact Or.inr stk
-                | inr eq => simp [hn, eq]
-            . apply And.intro
-              . intro i j mem step
-                rw [NodeSet.get_set] at mem
-                split at mem
-                case inl eq => simp [eq.symm, Node.εStep] at step
-                case inr neq =>
-                  have := inv₀.2.1 i j mem step
-                  cases this with
-                  | inl vis => simp [NodeSet.get_set_set vis]
-                  | inr stk =>
-                    cases decEq j n with
-                    | isTrue eq => simp [eq]
-                    | isFalse neq =>
-                      apply Or.inr
-                      apply Array.mem_pop _ _ _ stk neq
-              . intro j mem
-                cases mem with
-                | inl vis =>
-                  cases decEq j n with
-                  | isTrue eq =>
-                    simp [eq]
-                    have : n ∈ stack := Array.mem_back' hemp
-                    exact inv₀.2.2 n (.inr this)
-                  | isFalse neq =>
-                    rw [NodeSet.get_set_ne] at vis
-                    . exact inv₀.2.2 j (.inl vis)
-                    . intro h
-                      exact neq (Fin.eq_of_val_eq h).symm
-                | inr stk =>
-                  have : j ∈ stack := Array.mem_of_mem_pop _ _ stk
-                  exact inv₀.2.2 j (.inr this)
-          have ih := go (visited.set n) stack.pop inv'
-          simp at ih
-          exact ih
-
-  have inv₀ : inv .empty #[i] := by
-    simp [inv]
-    exact .base
-  let ⟨h₁, h₂, h₃⟩ := go .empty #[i] inv₀
-  simp at h₁ h₂ h₃
-  intro j
-  apply Iff.intro
-  . exact h₃ j
-  . intro h
-    let S := { j | ∃ j', (εClosureTR nfa inBounds .empty #[i]).get j' ∧ j = j'.val }
-    have mem : i.val ∈ S := by
-      simp
-      exact ⟨i, h₁, rfl⟩
-    have : ∀ j ∈ S, (_ : j < nfa.nodes.size) → ∀ k ∈ nfa[j].εStep, k ∈ S := by
-      intro j mem _ k step
-      simp at mem
-      let ⟨j', h₄, h₅⟩ := mem
-      simp [h₅] at step
-      have klt : k < nfa.nodes.size := lt_of_inBounds_of_εStep inBounds step
-      have := h₂ j' ⟨k, klt⟩ h₄ step
-      simp
-      exact ⟨⟨k, klt⟩, this, rfl⟩
-
-    have := mem_εStep_iff_εClosure_sub.mp this i mem
-    have := Set.mem_of_mem_of_subset h this
-    simp at this
-    let ⟨j', h₄, h₅⟩ := this
-    have : j = j' := Fin.eq_of_val_eq h₅
-    exact this ▸ h₄
-termination_by go _ => (visited.count_unset, stack.size)
-
-theorem charStepTR_spec {nfa : NFA} {inBounds : nfa.inBounds}
-  {init : NodeSet nfa.nodes.size} {k : Fin nfa.nodes.size} :
-  (charStepTR nfa inBounds c init).get k ↔
-  k.val ∈ nfa.stepSet { j | ∃ j', init.get j' ∧ j = j'.val } c := by
-  let inv (accum : NodeSet nfa.nodes.size) (i : Nat) : Prop :=
-    ∀ k, accum.get k ↔ k.val ∈ nfa.stepSet { j | ∃ j', init.get j' ∧ j'.val < i ∧ j = j'.val } c
-
-  let lem (i : Nat) (hlt : i < nfa.nodes.size) :
-    { j | ∃ j', init.get j' ∧ j' < i + 1 ∧ j = j'.val } =
-    if init.get ⟨i, hlt⟩ then
-      { j | ∃ j', init.get j' ∧ j' < i ∧ j = j'.val } ∪ {i}
-    else
-      { j | ∃ j', init.get j' ∧ j' < i ∧ j = j'.val } := by
-    split
-    case inl h =>
-      apply Set.eq_of_subset_of_subset
-      . intro j
-        simp
-        intro j' mem lt eq
-        have : j'.val ≤ i := Nat.le_of_lt_succ lt
-        cases Nat.lt_or_eq_of_le this with
-        | inl lt' => exact .inr ⟨j', mem, lt', eq⟩
-        | inr eq' => exact .inl (eq' ▸ eq)
-      . intro j
-        simp
-        intro h'
-        match h' with
-        | .inl eq =>
-          subst eq
-          exact ⟨⟨j, hlt⟩, h, Nat.lt_succ_self _, rfl⟩
-        | .inr ⟨j', mem, lt, eq⟩ => exact ⟨j', mem, Nat.lt_trans lt (Nat.lt_succ_self _), eq⟩
-    case inr h =>
-      apply Set.eq_of_subset_of_subset
-      . intro j
-        simp
-        intro j' mem lt eq
-        have : j'.val ≤ i := Nat.le_of_lt_succ lt
-        cases Nat.lt_or_eq_of_le this with
-        | inl lt' => exact ⟨j', mem, lt', eq⟩
-        | inr eq' =>
-          have : j' = ⟨i, hlt⟩ := Fin.eq_of_val_eq eq'
-          rw [this] at mem
-          contradiction
-      . intro j
-        simp
-        intro j' mem lt eq
-        exact ⟨j', mem, Nat.lt_trans lt (Nat.lt_succ_self _), eq⟩
-
-  let rec go (accum : NodeSet nfa.nodes.size) (i : Nat) (hle : i ≤ nfa.nodes.size)
-    (inv₀ : inv accum i) :
-    ∀ k, (charStepTR.go nfa inBounds c init accum i hle).get k ↔
-      k.val ∈ nfa.stepSet { j | ∃ j', init.get j' ∧ j = j'.val } c := by
-    unfold charStepTR.go
-    cases decEq i nfa.nodes.size with
-    | isTrue h =>
-      simp [h]
-      simp [h] at inv₀
-      exact inv₀
-    | isFalse h =>
-      simp [h]
-      have hlt : i < nfa.nodes.size := Nat.lt_of_le_of_ne hle h
-      cases hset : init.get ⟨i, hlt⟩ with
-      | true =>
-        simp
-        split
-        next c' next hn =>
-          split
-          case inl eq =>
-            have : next < nfa.nodes.size := by
-              have := inBounds ⟨i, hlt⟩
-              simp [Node.inBounds, hn] at this
-              exact this
-            set εCls := εClosureTR nfa inBounds .empty #[⟨next, this⟩]
-            set accum' := accum.merge εCls
-            have inv' : inv accum' (i + 1) := by
-              simp [lem i hlt, hset]
-              simp [stepSet_insert_distrib, NodeSet.merge_get]
-              intro k
-              apply Iff.or
-              . exact inv₀ k
-              . rw [εClosureTR_spec k]
-                simp [NFA.stepSet, getElem?_pos nfa i hlt, hn, Option.charStep, Node.charStep, eq]
-                simp [NFA.εClosureSet]
-            exact go accum' (i + 1) hlt inv'
-          case inr neq =>
-            have inv' : inv accum (i + 1) := by
-              simp [lem i hlt, hset]
-              have : nfa.stepSet {i} c = ∅ := by
-                simp [NFA.stepSet, getElem?_pos nfa i hlt, hn, Option.charStep, Node.charStep, neq]
-              simp [stepSet_insert_distrib, this]
-              exact inv₀
-            exact go accum (i + 1) hlt inv'
-        next hn =>
-          have inv' : inv accum (i + 1) := by
-            simp [lem i hlt, hset]
-            have : nfa.stepSet {i} c = ∅ := by
-              simp [NFA.stepSet, getElem?_pos nfa i hlt, hn, Option.charStep, Node.charStep]
-            simp [stepSet_insert_distrib, this]
-            exact inv₀
-          exact go accum (i + 1) hlt inv'
-      | false =>
-        simp
-        have inv' : inv accum (i + 1) := by
-          simp [lem i hlt, hset]
-          exact inv₀
-        exact go accum (i + 1) hlt inv'
-
-  have inv₀ : inv .empty 0 := by simp [inv, Nat.not_lt_zero]
-  apply go .empty 0 (Nat.zero_le _) inv₀
-termination_by go _ => nfa.nodes.size - i
-
-def matchList (nfa : NFA) (inBounds : nfa.inBounds) (cs : List Char) : Bool :=
-  let ns := εClosureTR nfa inBounds .empty #[nfa.start]
-  let ns := go nfa inBounds cs ns
-  -- This assumes that the first node is the accepting node
-  ns.get ⟨0, nfa.zero_lt_size⟩
-where
-  go (nfa : NFA) (inBounds : nfa.inBounds) (cs : List Char) (ns : NodeSet nfa.nodes.size) :
-    NodeSet nfa.nodes.size :=
-    List.foldl (fun ns c => charStepTR nfa inBounds c ns) ns cs
-
-theorem matchList.go_eq_foldl_stepSet {nfa : NFA} {ns : NodeSet nfa.nodes.size}
-  {inBounds : nfa.inBounds} {cs : List Char} :
-  ∀ j, (go nfa inBounds cs ns).get j ↔
-    j.val ∈ List.foldl nfa.stepSet { i | ∃ i', ns.get i' ∧ i = i'.val } cs := by
-  induction cs generalizing ns with
-  | nil =>
-    simp [go]
-    intro j
-    apply Iff.intro
-    . intro h
-      exact ⟨j, h, rfl⟩
-    . intro h
-      let ⟨j', h₁, h₂⟩ := h
-      rw [Fin.eq_of_val_eq h₂, h₁]
-  | cons c cs ih =>
-    simp [go]
-    unfold go at ih
-    set ns' := charStepTR nfa inBounds c ns
-    have spec : ∀ k, ns'.get k ↔ k.val ∈ nfa.stepSet { i | ∃ i', ns.get i' ∧ i = i'.val } c := by
-      intro k
-      exact charStepTR_spec
-    intro j
-    rw [ih j]
-    congr!
-    apply Set.eq_of_subset_of_subset
-    . intro i
-      simp
-      intro i' mem eq
-      exact eq ▸ (spec i').mp mem
-    . intro i mem
-      simp
-      have lt : i < nfa.nodes.size := lt_of_inBounds_of_stepSet inBounds mem
-      have := (spec ⟨i, lt⟩).mpr mem
-      exact ⟨⟨i, lt⟩, this, rfl⟩
-
-theorem match.go_eq_matchList.go {nfa : NFA} {inBounds : nfa.inBounds} {ns : NodeSet nfa.nodes.size}
-  {it : String.Iterator} {cs cs' : List Char} (v : it.ValidFor cs cs') :
-  NFA.match.go nfa inBounds it ns = matchList.go nfa inBounds cs' ns := by
-  induction cs' generalizing it cs ns with
-  | nil =>
-    unfold NFA.match.go matchList.go
-    have : it.atEnd := v.atEnd.mpr rfl
-    simp [this]
-  | cons c cs' ih =>
-    unfold NFA.match.go matchList.go
-    have : ¬ it.atEnd := by
-      intro h
-      have := v.atEnd.mp h
-      contradiction
-    simp [this]
-    have : it.curr = c := by
-      simp [v.curr]
-    simp [this]
-    exact ih v.next
-
-theorem evalFrom_iff_matchList {nfa : NFA} {inBounds : nfa.inBounds} {cs : List Char} :
-  0 ∈ nfa.evalFrom {nfa.start.val} cs ↔ matchList nfa inBounds cs := by
-  unfold NFA.evalFrom matchList
-  simp [matchList.go_eq_foldl_stepSet, εClosureTR_spec]
-  have :
-    {i | ∃ i' : Fin nfa.nodes.size, i'.val ∈ NFA.εClosure nfa nfa.start.val ∧ i = i'.val} =
-    nfa.εClosureSet {nfa.start.val} := by
-    simp [NFA.εClosureSet]
-    apply Set.eq_of_subset_of_subset
-    . intro i mem
-      simp at mem
-      let ⟨i', mem', eq⟩ := mem
-      exact eq ▸ mem'
-    . intro i mem
-      have lt : i < nfa.nodes.size := lt_of_inBounds_of_εClosure inBounds nfa.start.isLt mem
-      simp
-      exact ⟨⟨i, lt⟩, mem, rfl⟩
-  rw [this]
-
-end NFA.VM
-
-namespace NFA
-
-theorem match_eq_matchList {nfa : NFA} {inBounds : nfa.inBounds} {s : String} :
-  NFA.match nfa inBounds s = NFA.VM.matchList nfa inBounds s.data := by
-  unfold NFA.match NFA.VM.matchList
-  simp
-  rw [NFA.VM.match.go_eq_matchList.go s.validFor_mkIterator]
-
--- Correctness of the VM interpreter
-theorem NFA.match_iff_regex_matches {s : String} (eq : compile r = nfa) :
-  nfa.match (compile.inBounds eq) s ↔ r.matches s := by
-  apply Iff.intro
-  . intro m
-    have : NFA.VM.matchList nfa (compile.inBounds eq) s.data :=
-      match_eq_matchList ▸ m
-    have := NFA.VM.evalFrom_iff_matchList.mpr this
-    exact matches_of_evalFrom' eq this
-  . intro m
-    have := evalFrom_of_matches' eq m
-    have := (NFA.VM.evalFrom_iff_matchList (inBounds := compile.inBounds eq)).mp this
-    exact match_eq_matchList ▸ this
-
-end NFA
-
-namespace NFAa.VM
-
-open NFA.VM
-
-theorem mem_εStep_iff_εClosure_sub {nfa : NFAa} {S : Set Nat} :
-  (∀ i ∈ S, (_ : i < nfa.nodes.size) → ∀ j ∈ nfa[i].εStep, j ∈ S) ↔
-  ∀ i ∈ S, nfa.εClosure i ⊆ S := by
-  apply Iff.intro
-  . intro assm i mem
     intro k cls
     induction cls with
     | base => exact mem
@@ -602,7 +92,7 @@ theorem mem_εStep_iff_εClosure_sub {nfa : NFAa} {S : Set Nat} :
     apply Set.mem_of_mem_of_subset _ (assm i mem)
     exact εClosure.step (εStep_of_εStep step) .base
 
-def εClosureTRa_spec.inv (nfa : NFAa) (i : Fin nfa.nodes.size)
+def εClosureTRa_spec.inv (nfa : NFA) (i : Fin nfa.nodes.size)
   (visited : NodeSet nfa.nodes.size) (stack : Array (Fin nfa.nodes.size)) : Prop :=
   (visited.get i ∨ i ∈ stack) ∧
   (∀ i j, visited.get i → j.val ∈ nfa[i].εStep → visited.get j ∨ j ∈ stack) ∧
@@ -786,7 +276,7 @@ theorem εClosureTRa_spec.case_else (inv₀ : inv nfa i visited stack)
       exact h₃ j (.inr this)
 
 -- The case analysis takes a bit of time, so we split each branch as lemmas
-theorem εClosureTRa_spec.go (nfa : NFAa) (i : Fin nfa.nodes.size) {visited stack}
+theorem εClosureTRa_spec.go (nfa : NFA) (i : Fin nfa.nodes.size) {visited stack}
   (inv₀ : inv nfa i visited stack) :
   inv nfa i (εClosureTRa nfa visited stack) #[] := by
   unfold εClosureTRa
@@ -806,7 +296,7 @@ theorem εClosureTRa_spec.go (nfa : NFAa) (i : Fin nfa.nodes.size) {visited stac
       next hn₁ hn₂ => exact go nfa i (case_else inv₀ hemp hvis hn₁ hn₂)
 termination_by _ => (visited.count_unset, stack.size)
 
-theorem εClosureTRa_spec {nfa : NFAa} {i : Fin nfa.nodes.size} :
+theorem εClosureTRa_spec {nfa : NFA} {i : Fin nfa.nodes.size} :
   ∀ j, (εClosureTRa nfa .empty #[i]).get j ↔ j.val ∈ nfa.εClosure i := by
   have inv₀ : εClosureTRa_spec.inv nfa i .empty #[i] := by
     simp [εClosureTRa_spec.inv]
@@ -835,11 +325,11 @@ theorem εClosureTRa_spec {nfa : NFAa} {i : Fin nfa.nodes.size} :
     simp at this
     exact this
 
-def charStepTRa_spec.inv (nfa : NFAa) (c : Char) (init : NodeSet nfa.nodes.size)
+def charStepTRa_spec.inv (nfa : NFA) (c : Char) (init : NodeSet nfa.nodes.size)
   (accum : NodeSet nfa.nodes.size) (i : Nat) : Prop :=
   ∀ k, accum.get k ↔ k.val ∈ nfa.stepSet { j | j < i ∧ ∃ h : j < nfa.nodes.size, init.get ⟨j, h⟩ } c
 
-theorem charStepTRa_spec.lem (nfa : NFAa) (init : NodeSet nfa.nodes.size)
+theorem charStepTRa_spec.lem (nfa : NFA) (init : NodeSet nfa.nodes.size)
   (i : Nat) (hlt : i < nfa.nodes.size) :
   { j | j < i + 1 ∧ ∃ h : j < nfa.nodes.size, init.get ⟨j, h⟩ } =
   if init.get ⟨i, hlt⟩ then
@@ -874,7 +364,7 @@ theorem charStepTRa_spec.lem (nfa : NFAa) (init : NodeSet nfa.nodes.size)
       intro lt₁ lt₂ hset'
       exact ⟨Nat.lt_trans lt₁ (Nat.lt_succ_self _), lt₂, hset'⟩
 
-theorem charStepTRa_spec.go (nfa : NFAa) (c : Char) (init : NodeSet nfa.nodes.size)
+theorem charStepTRa_spec.go (nfa : NFA) (c : Char) (init : NodeSet nfa.nodes.size)
   (accum : NodeSet nfa.nodes.size) (i : Nat) (hle : i ≤ nfa.nodes.size)
   (inv₀ : inv nfa c init accum i) :
   ∀ k, ((charStepTRa.go nfa c init accum i hle)).get k ↔
@@ -941,23 +431,23 @@ theorem charStepTRa_spec.go (nfa : NFAa) (c : Char) (init : NodeSet nfa.nodes.si
       exact inv₀
 termination_by _ => nfa.nodes.size - i
 
-theorem charStepTRa_spec (nfa : NFAa) (c : Char) (init : NodeSet nfa.nodes.size) :
+theorem charStepTRa_spec (nfa : NFA) (c : Char) (init : NodeSet nfa.nodes.size) :
   ∀ k, (charStepTRa nfa c init).get k ↔
   k.val ∈ nfa.stepSet { j | ∃ h : j < nfa.nodes.size, init.get ⟨j, h⟩ } c := by
   have inv₀ : charStepTRa_spec.inv nfa c init .empty 0 := by
     simp [charStepTRa_spec.inv, Nat.not_lt_zero]
   exact charStepTRa_spec.go nfa c init .empty 0 (Nat.zero_le _) inv₀
 
-def matchList (nfa : NFAa) (cs : List Char) : Bool :=
+def matchList (nfa : NFA) (cs : List Char) : Bool :=
   let ns := εClosureTRa nfa .empty #[nfa.start]
   let ns := go nfa cs ns
   -- This assumes that the first node is the accepting node
   ns.get ⟨0, nfa.zero_lt_size⟩
 where
-  go (nfa : NFAa) (cs : List Char) (ns : NodeSet nfa.nodes.size) : NodeSet nfa.nodes.size :=
+  go (nfa : NFA) (cs : List Char) (ns : NodeSet nfa.nodes.size) : NodeSet nfa.nodes.size :=
     List.foldl (fun ns c => charStepTRa nfa c ns) ns cs
 
-theorem matchList.go_eq_foldl_stepSet {nfa : NFAa} {ns : NodeSet nfa.nodes.size} {cs : List Char} :
+theorem matchList.go_eq_foldl_stepSet {nfa : NFA} {ns : NodeSet nfa.nodes.size} {cs : List Char} :
   ∀ j, (go nfa cs ns).get j ↔
     j.val ∈ List.foldl nfa.stepSet { i | ∃ h : i < nfa.nodes.size, ns.get ⟨i, h⟩ } cs := by
   induction cs generalizing ns with
@@ -977,9 +467,9 @@ theorem matchList.go_eq_foldl_stepSet {nfa : NFAa} {ns : NodeSet nfa.nodes.size}
       simp [mem]
       exact lt_of_mem_stepSet mem
 
-theorem evalFrom_iff_matchList {nfa : NFAa} {cs : List Char} :
+theorem evalFrom_iff_matchList {nfa : NFA} {cs : List Char} :
   0 ∈ nfa.evalFrom {nfa.start.val} cs ↔ matchList nfa cs := by
-  unfold NFAa.evalFrom matchList
+  unfold NFA.evalFrom matchList
   simp [matchList.go_eq_foldl_stepSet, εClosureTRa_spec]
   congr! 2
   simp [εClosureSet]
@@ -991,16 +481,16 @@ theorem evalFrom_iff_matchList {nfa : NFAa} {cs : List Char} :
     simp at mem
     exact mem.right
 
-theorem match.go_eq_matchList.go {nfa : NFAa} {ns : NodeSet nfa.nodes.size}
+theorem match.go_eq_matchList.go {nfa : NFA} {ns : NodeSet nfa.nodes.size}
   {it : String.Iterator} {cs cs' : List Char} (v : it.ValidFor cs cs') :
-  NFAa.match.go nfa it ns = matchList.go nfa cs' ns := by
+  NFA.match.go nfa it ns = matchList.go nfa cs' ns := by
   induction cs' generalizing it cs ns with
   | nil =>
-    unfold NFAa.match.go matchList.go
+    unfold NFA.match.go matchList.go
     have : it.atEnd := v.atEnd.mpr rfl
     simp [this]
   | cons c cs' ih =>
-    unfold NFAa.match.go matchList.go
+    unfold NFA.match.go matchList.go
     have : ¬ it.atEnd := by
       intro h
       have := v.atEnd.mp h
@@ -1011,19 +501,19 @@ theorem match.go_eq_matchList.go {nfa : NFAa} {ns : NodeSet nfa.nodes.size}
     simp [this]
     exact ih v.next
 
-theorem match_eq_matchList {nfa : NFAa} {s : String} :
+theorem match_eq_matchList {nfa : NFA} {s : String} :
   nfa.match s ↔ matchList nfa s.data := by
-  unfold NFAa.match matchList
+  unfold NFA.match matchList
   simp
   rw [match.go_eq_matchList.go s.validFor_mkIterator]
 
-theorem evalFrom_iff_match {nfa : NFAa} {s : String} :
+theorem evalFrom_iff_match {nfa : NFA} {s : String} :
   nfa.match s ↔ 0 ∈ nfa.evalFrom {nfa.start.val} s.data := by
   rw [match_eq_matchList, evalFrom_iff_matchList]
 
-theorem match_iff_regex_matches (eq : NFAa.compile r = nfa) :
+theorem match_iff_regex_matches (eq : NFA.compile r = nfa) :
   nfa.match s ↔ r.matches s := by
   rw [evalFrom_iff_match]
   exact ⟨matches_of_compile_evalFrom eq, evalFrom_of_compile_matches eq⟩
 
-end NFAa.VM
+end NFA.VM
