Regex/NFA/Tests.lean
@@ -2,23 +2,23 @@ import Regex.NFA.Compile
 import Regex.NFA.VM
 
 def r₁ := Regex.concat (Regex.star (Regex.char 'a')) (Regex.star (Regex.char 'b'))
-def NFA₁ := NFAa.compile r₁
+def NFA₁ := NFA.compile r₁
 #eval NFA₁.match "aaaabbbb"
 #eval NFA₁.match "ab"
 #eval NFA₁.match "c"
 #eval NFA₁.match ""
 
 def r₂ := Regex.star (Regex.alternate (Regex.star (Regex.char 'a')) (Regex.char 'b'))
-def NFA₂ := NFAa.compile r₂
+def NFA₂ := NFA.compile r₂
 #eval NFA₂.match "aaaabbbb"
 #eval NFA₂.match "abcab"
 #eval NFA₂.match ""
 
-def NFA₃ := NFAa.compile (Regex.alternate Regex.empty (Regex.concat (Regex.char 'a') Regex.empty))
+def NFA₃ := NFA.compile (Regex.alternate Regex.empty (Regex.concat (Regex.char 'a') Regex.empty))
 #eval NFA₃.match ""
 #eval NFA₃.match "a"
 
-def NFA₄ := NFAa.compile (Regex.concat (Regex.alternate (Regex.char 'a') (Regex.char 'b')) (Regex.char 'c'))
+def NFA₄ := NFA.compile (Regex.concat (Regex.alternate (Regex.char 'a') (Regex.char 'b')) (Regex.char 'c'))
 #eval NFA₄.match "ac"
 #eval NFA₄.match "bc"
 #eval NFA₄.match "a"
