RegexCorrectness/NFA/Transition/MatchOfAccept.lean
@@ -1,7 +1,7 @@
 -- When the compiled NFA accepts a prefix, the regex matches it.
 import RegexCorrectness.NFA.Transition.Basic
 
-namespace NFAa
+namespace NFA
 
 theorem eq_next_of_pathToNext (eq : pushRegex nfa next r = result)
   (assm : next' < nfa.nodes.size)
@@ -409,14 +409,14 @@ theorem matches_prefix_of_path (eq : pushRegex nfa next r = result)
   | concat r₁ r₂ ih₁ ih₂ => exact matches_prefix_of_path.concat eq path ih₁ ih₂
   | star r ih => exact matches_prefix_of_path.star eq path ih
 
-theorem matches_prefix_of_compile_path (eq : NFAa.compile r = nfa)
+theorem matches_prefix_of_compile_path (eq : NFA.compile r = nfa)
   (path : pathToNext nfa 0 1 nfa.start.val s s') :
   ∃ p, s = p ++ s' ∧ r.matches ⟨p⟩ := by
-  set result := NFAa.done.pushRegex ⟨0, by decide⟩ r
+  set result := NFA.done.pushRegex ⟨0, by decide⟩ r
   have : nfa = result.val := by
     rw [←eq]
     rfl
   rw [this] at path
   exact matches_prefix_of_path rfl path
 
-end NFAa
+end NFA
